HoTTModel/DTT/SynCat.lean
@@ -1,0 +1,558 @@
+import HoTTModel.DTT.PTS
+import HoTTModel.Contextual
+
+namespace PureTypeSystem
+
+open Classical CategoryTheory Limits
+
+noncomputable section TermModel
+
+@[ext]
+structure Ctx (S : Specification) where
+  ctx : PCtx S
+  wf : Nonempty (ctx ⊢ ⬝)
+
+def PCtx.cons (Γ : PCtx S) (A : PTerm S) (h : Nonempty (A :: Γ ⊢ ⬝)) : Ctx S where
+  ctx := A :: Γ
+  wf := h
+
+namespace Ctx
+
+def wf' (Γ : Ctx S) : Γ.ctx ⊢ ⬝ := choice Γ.wf
+
+def betac (Γ Δ : Ctx S) : Prop := Nonempty (Γ.ctx ≃β Δ.ctx)
+
+lemma betac.equivalence :
+    Equivalence (betac (S := S)) where
+  refl Γ := ⟨PCtx.betac.refl Γ.ctx⟩
+  symm := by intro _ _ ⟨h₁⟩; exact ⟨h₁.symm⟩
+  trans := by intro _ _ _ ⟨h₁⟩ ⟨h₂⟩; exact ⟨h₁.trans _ _ _ h₂⟩
+
+instance setoid (S : Specification) : Setoid (Ctx S) where
+  iseqv := betac.equivalence
+
+abbrev nil : Ctx S := ⟨[], ⟨wf.nil⟩⟩
+
+lemma eq_nil_of_equiv_nil {Γ : Ctx S} :
+    Γ ≈ nil → Γ = nil := by
+  intro ⟨h⟩; ext
+  simpa using h.length_eq
+
+def tail : (Γ : Ctx S) → Ctx S
+| .mk [] _ => nil
+| .mk (_ :: Γ) h => ⟨Γ, ⟨wf_of_cons (choice h)⟩⟩
+
+@[simp]
+lemma tail_eq_list_tail : ∀ (Γ : Ctx S), Γ.tail.ctx = Γ.ctx.tail
+| .mk [] _ => rfl
+| .mk (_ :: _) _ => rfl
+
+lemma tail_sound {Γ Δ : Ctx S} : (h : Γ ≈ Δ) → Γ.tail ≈ Δ.tail := by
+  intro ⟨h⟩
+  constructor
+  simpa using h.tail'
+
+@[simp]
+lemma nil_tail : (nil : Ctx S).tail = nil := rfl
+
+end Ctx
+
+def QCtx (S : Specification) := Quotient (Ctx.setoid S)
+
+notation:1024 "[" Γ "]ᵣ"=> Ctx.ctx (Quotient.out Γ)
+
+section
+
+lemma Ctx.mk_out_equiv (Γ : Ctx S) : (⟦Γ⟧ : QCtx S).out ≈ Γ :=
+  Quotient.mk_out _
+
+def Ctx.mk_rep_betac (Γ : Ctx S) : [(⟦Γ⟧ : QCtx S)]ᵣ ≃β Γ.ctx :=
+  choice Γ.mk_out_equiv
+
+lemma QCtx.out_mk_eq (Γ : QCtx S) : ⟦(⟨[Γ]ᵣ, Γ.out.wf⟩ : Ctx S)⟧ = Γ :=
+  Quotient.out_eq Γ
+
+end
+
+namespace QCtx
+
+def wf (Γ : QCtx S) : [Γ]ᵣ ⊢ ⬝ := choice Γ.out.wf
+
+structure hom₀ (Γ Δ : Ctx S) where
+  seq : PCtx S
+  is : Nonempty (isMor Γ.ctx Δ.ctx seq)
+
+def _root_.PureTypeSystem.Ctx.proj : (Γ : Ctx S) → hom₀ Γ Γ.tail
+| .mk [] _ => ⟨[], ⟨isMor.nil⟩⟩
+| .mk (_ :: Γ) h => {
+  seq := id₀ 1 Γ
+  is := ⟨id_isMor (isTrunc.succ _ (isTrunc.zero _)) (choice h)⟩
+}
+
+namespace hom₀
+
+def betac {Γ Δ : Ctx S} (γ δ : hom₀ Γ Δ) : Prop := Nonempty (γ.seq ≃β δ.seq)
+
+lemma betac.equivalence :
+    Equivalence (@betac _ Γ Δ) where
+  refl δ := ⟨PCtx.betac.refl δ.seq⟩
+  symm := by intro _ _ ⟨h₁⟩; exact ⟨h₁.symm⟩
+  trans := by intro _ _ _ ⟨h₁⟩ ⟨h₂⟩; exact ⟨h₁.trans _ _ _ h₂⟩
+
+instance setoid (Γ Δ : Ctx S) : Setoid (hom₀ Γ Δ) where
+  iseqv := betac.equivalence
+
+end hom₀
+
+def hom (Γ Δ : QCtx S) : Type _ := Quotient (hom₀.setoid Γ.out Δ.out)
+
+notation:1024 "[" γ "]ᵣ" => hom₀.seq (Quotient.out γ)
+
+lemma hom₀.mk_out_equiv {Γ Δ : QCtx S} (δ : hom₀ Γ.out Δ.out) : (⟦δ⟧ : hom _ _).out ≈ δ :=
+  Quotient.mk_out _
+
+def hom₀.mk_rep_betac {Γ Δ : QCtx S} (δ : hom₀ Γ.out Δ.out) : [(⟦δ⟧ : hom _ _)]ᵣ ≃β δ.seq :=
+  choice δ.mk_out_equiv
+
+lemma hom.out_mk_eq {Γ Δ : QCtx S} (δ : hom Γ Δ) : ⟦(⟨[δ]ᵣ, δ.out.is⟩ : hom₀ _ _)⟧ = δ :=
+  Quotient.out_eq δ
+
+def hom.is (γ : hom Γ Δ) : isMor [Γ]ᵣ [Δ]ᵣ [γ]ᵣ := choice γ.out.is
+
+protected def id₀ (Γ : QCtx S) : hom₀ Γ.out Γ.out where
+  seq := id₀ 0 [Γ]ᵣ
+  is := ⟨id_isMor (isTrunc.zero _) Γ.wf⟩
+
+protected def id (Γ : QCtx S) : hom Γ Γ := ⟦Γ.id₀⟧
+
+def id_rep_betac (Γ : QCtx S) : [Γ.id]ᵣ ≃β (id [Γ]ᵣ) :=
+  hom₀.mk_rep_betac _
+
+def comp₀ {Γ Δ Θ : QCtx S} (γ : hom Γ Δ) (δ : hom Δ Θ) :
+    hom₀ Γ.out Θ.out :=
+  { seq := pcomp [γ]ᵣ [δ]ᵣ
+    is := ⟨pcomp_isMor Γ.wf Θ.wf γ.is δ.is⟩
+  }
+
+def comp {Γ Δ Θ : QCtx S} (γ : hom Γ Δ) (δ : hom Δ Θ) :
+    hom Γ Θ := ⟦comp₀ γ δ⟧
+
+instance : Category (QCtx S) where
+  Hom := hom
+  id := QCtx.id
+  comp := comp
+  id_comp {Γ Δ} f := by
+    rw [← Quotient.out_equiv_out]
+    constructor
+    sorry
+  comp_id {Γ Δ} f := by
+    rw [← Quotient.out_equiv_out]
+    constructor
+    simp [comp]
+    refine (hom₀.mk_rep_betac _).trans _ _ _ ((pcomp_betac₂ Δ.id_rep_betac).trans _ _ _ ?_)
+    rw [pcomp_id f.is]
+    apply PCtx.betac.refl _
+  assoc := sorry
+
+def one : QCtx S := ⟦Ctx.nil⟧
+
+@[simp]
+lemma one_rep_length : [(one : QCtx S)]ᵣ.length = 0 :=
+  Ctx.nil.mk_rep_betac.length_eq
+
+@[simp]
+lemma one_rep : [(one : QCtx S)]ᵣ = [] := by
+  rw [← List.length_eq_zero]
+  apply one_rep_length
+
+lemma eq_one_iff_rep_length_eq_zero (Γ : QCtx S) :
+    Γ = one ↔ [Γ]ᵣ.length = 0 := by
+  constructor
+  . intro h; simp only [h, one_rep, List.length_nil]
+  . intro h
+    rw [← Γ.out_mk_eq]
+    simp at h
+    simp [h, one]
+
+def hom_one (Γ : QCtx S) : Γ ⟶ one := by
+  apply Quotient.mk' {
+    seq := []
+    is := ⟨by simpa using isMor.nil⟩
+  }
+
+lemma hom.eq_iff_nonempty_rep_betac {Γ Δ : QCtx S} {γ δ : Γ ⟶ Δ} :
+    γ = δ ↔  Nonempty ([γ]ᵣ ≃β [δ]ᵣ) := by
+  rw [← Quotient.out_equiv_out]
+  rfl
+
+@[simp]
+lemma hom_one_rep_eq_nil (Γ : QCtx S) (h : Γ ⟶ one) : [h]ᵣ = [] := by
+  obtain ⟨is⟩ := h.out.is
+  simp at is
+  exact is.of_nil
+
+lemma hom_one_uniq (Γ : QCtx S) (h : Γ ⟶ one) : h = Γ.hom_one := by
+  rw [hom.eq_iff_nonempty_rep_betac]
+  simp
+  exact ⟨PCtx.betac.refl _⟩
+
+def ft (Γ : QCtx S) : QCtx S := ⟦Γ.out.tail⟧
+
+def ft_rep_betac_rep_tail (Γ : QCtx S) :
+    [Γ.ft]ᵣ ≃β [Γ]ᵣ.tail := by
+  rw [← Γ.out.tail_eq_list_tail]
+  exact Γ.out.tail.mk_rep_betac
+
+def ft_mk_cons_rep_betac (Γ : PCtx S) (A : PTerm S) (h : Nonempty (A :: Γ ⊢ ⬝)) :
+    [ft ⟦Γ.cons A h⟧]ᵣ ≃β Γ :=
+  (ft_rep_betac_rep_tail ⟦Γ.cons A h⟧).trans _ _ _
+    ((Γ.cons A h).mk_rep_betac.tail')
+
+def proj₀ (Γ : Ctx S) : hom ⟦Γ⟧ (ft ⟦Γ⟧) := Quotient.mk' {
+  seq := id₀ 1 Γ.ctx.tail
+  is := ⟨isMor_betac Γ.wf' (Ctx.wf' _) (Ctx.wf' _) Γ.mk_rep_betac.symm
+      ((Γ.mk_rep_betac.tail'.symm).trans _ _ _ (ft_rep_betac_rep_tail _).symm)
+      (id_isMor_tail Γ.wf')⟩
+}
+
+lemma test {Γ Δ : QCtx S} {f : Γ ⟶ Δ} {g : Γ ⟶ Δ} (h : [f]ᵣ ≃β [g]ᵣ) :
+    f = g := by
+  rw [← Quotient.out_equiv_out]
+  exact ⟨h⟩
+
+lemma test' {Γ Γ' Δ Δ' : QCtx S} (h₁ : Γ = Γ') (h₂ : Δ = Δ')
+  {f : Γ ⟶ Δ} {f' : Γ' ⟶ Δ'} (h : [f]ᵣ ≃β [f']ᵣ) :
+      HEq f f' := by
+  cases h₁; cases h₂; simp only [heq_eq_eq]
+  apply test h
+
+lemma proj₀_sound (Γ Δ : Ctx S) (h : Γ ≈ Δ) : HEq (proj₀ Γ) (proj₀ Δ) := by
+  apply test' (Quotient.sound h) (congrArg _ (Quotient.sound h))
+  refine ((hom₀.mk_rep_betac _).trans _ _ _ ?_).trans _ _ _ ((hom₀.mk_rep_betac _).symm)
+  simp only [Ctx.tail_eq_list_tail, id₀]
+  convert PCtx.betac.refl _ using 2
+  simp [(choice h).length_eq]
+
+def proj (Γ : QCtx S) : Γ ⟶ Γ.ft :=
+  Quotient.hrecOn (motive := fun Γ : QCtx S ↦ Γ ⟶ Γ.ft) _ _ proj₀_sound
+
+instance instPreContextualCategory : PreContextualCategory (QCtx S) where
+  gr Γ := [Γ]ᵣ.length
+  one := one
+  one_gr := one_rep_length
+  one_uniq := by intros; rwa [eq_one_iff_rep_length_eq_zero]
+  one_terminal := IsTerminal.ofUniqueHom (fun Γ ↦ hom_one Γ) hom_one_uniq
+  ft := ft
+  ft_one := by
+    simp [one, ft, Quotient.sound (Ctx.tail_sound (Ctx.nil.mk_out_equiv))]
+  ft_gr := by
+    intro n Γ h
+    simp at h ⊢
+    rw [Γ.ft_rep_betac_rep_tail.length_eq, List.length_tail, h,
+      Nat.add_one_sub_one]
+  proj := proj
+
+open PreContextualCategory
+
+lemma false_of_NR_one (h : NR (one : QCtx S)) : False := by
+  have := h.nr
+  erw [one_gr] at this
+  trivial
+
+instance (Γ : PCtx S) (A : PTerm S) (h : Nonempty (A :: Γ ⊢ ⬝)) :
+    @NR _ instPreContextualCategory ⟦Γ.cons A h⟧ where
+  nr := by simp only [gr]; rw [(Γ.cons A h).mk_rep_betac.length_eq]; simp [PCtx.cons]
+
+lemma NR_cons_iff_true (Γ : PCtx S) (A : PTerm S) (h : Nonempty (A :: Γ ⊢ ⬝)) :
+    @NR _ instPreContextualCategory ⟦Γ.cons A h⟧ ↔ True := by
+  simp only [iff_true]; infer_instance
+
+lemma NR_cons_iff_true' (Γ : PCtx S) (A : PTerm S) (h : Nonempty (A :: Γ ⊢ ⬝)) :
+    @NR _ instPreContextualCategory ⟦{ctx := A :: Γ, wf := h}⟧ ↔ True := by
+  apply NR_cons_iff_true _ _ h
+
+def cases_cons' {motive : (Γ : Ctx S) → [@NR _ instPreContextualCategory ⟦Γ⟧] → Sort w}
+  (h : ∀ (Γ : PCtx S) (A : PTerm S) (h : Nonempty (A :: Γ ⊢ ⬝)), motive (Γ.cons A h)) :
+    ∀ (Γ : Ctx S) [@NR _ instPreContextualCategory ⟦Γ⟧], motive Γ
+| .mk [] _, h => by simpa using false_of_NR_one h
+| .mk (A :: Γ) h₀, h₁ => h Γ A  h₀
+
+lemma auxheq {α β : Sort u} {a : α} {b : β} (h : HEq a b) :
+    HEq α β := by
+  cases h; rfl
+
+lemma heq_prop_ext (A B : Prop) (U : A → Sort u) (F : (a : A) → U a)
+  (V : B → Sort u) (G : (b : B) → V b) (a : A) (b : B) (h : HEq (F a) (G b)) :
+    HEq F G := by
+  have h₀ : A ↔ B :=
+    ⟨fun _ ↦ b, fun _ ↦ a⟩
+  simp only [← eq_iff_iff] at h₀
+  cases h₀
+  have : a = b := rfl
+  cases this
+  have h' : HEq (U a) (V a) := by
+    apply auxheq h
+  simp at h'
+  have : U = V := by ext; exact h'
+  cases this
+  simp at h ⊢
+  ext; exact h
+
+lemma cases_cons_aux {motive : (Γ : QCtx S) → [NR Γ] → Sort w}
+  (h : ∀ (Γ : PCtx S) (A : PTerm S) (h : Nonempty (A :: Γ ⊢ ⬝)), motive ⟦Γ.cons A h⟧)
+  (h' : ∀ (Γ Δ : PCtx S) (A B : PTerm S) (h₁ : Nonempty (A :: Γ ⊢ ⬝))
+    (h₂ : Nonempty (B :: Δ ⊢ ⬝)), Γ.cons A h₁ ≈ Δ.cons B h₂ → HEq (h Γ A h₁) (h Δ B h₂)) :
+  ∀ (Γ Δ : Ctx S), Γ ≈ Δ →
+    HEq (@cases_cons' S (fun x ↦ @motive ⟦x⟧) h Γ) (@cases_cons' S (fun x ↦ @motive ⟦x⟧) h Δ)
+| .mk [] _, b, h₁ => by cases Ctx.eq_nil_of_equiv_nil (Setoid.symm h₁); rfl
+| a, .mk [] _, h₁ => by cases Ctx.eq_nil_of_equiv_nil h₁; rfl
+| .mk (A :: Γ) h₀, .mk (B :: Δ) h₁, h₂ => by
+  apply heq_prop_ext
+  apply h' Γ Δ A B h₀ h₁ h₂
+
+@[elab_as_elim]
+def cases_cons {motive : (Γ : QCtx S) → [NR Γ] → Sort w}
+  (h : ∀ (Γ : PCtx S) (A : PTerm S) (h : Nonempty (A :: Γ ⊢ ⬝)), motive ⟦Γ.cons A h⟧)
+  (h' : ∀ (Γ Δ : PCtx S) (A B : PTerm S) (h₁ : Nonempty (A :: Γ ⊢ ⬝))
+    (h₂ : Nonempty (B :: Δ ⊢ ⬝)), Γ.cons A h₁ ≈ Δ.cons B h₂ → HEq (h Γ A h₁) (h Δ B h₂))
+  (Γ : QCtx S) [NR Γ] :
+    motive Γ :=
+  Quotient.hrecOn (motive := fun Γ : QCtx S ↦ ([NR Γ] → motive Γ)) _ (cases_cons' h)
+    (cases_cons_aux h h')
+
+/-
+-- interesting..
+lemma cases_cons_spec {motive : (Γ : QCtx S) → [NR Γ] → Sort w}
+  (h : ∀ (Γ : PCtx S) (A : PTerm S) (h : Nonempty (A :: Γ ⊢ ⬝)), motive ⟦Γ.cons A h⟧)
+  (h' : ∀ (Γ Δ : PCtx S) (A B : PTerm S) (h₁ : Nonempty (A :: Γ ⊢ ⬝))
+    (h₂ : Nonempty (B :: Δ ⊢ ⬝)), Γ.cons A h₁ ≈ Δ.cons B h₂ → HEq (h Γ A h₁) (h Δ B h₂))
+  (Γ : PCtx S) (A : PTerm S) (hΓ : Nonempty (A :: Γ ⊢ ⬝)) :
+    (@cases_cons S motive h h' ⟦Γ.cons A hΓ⟧ _) = h Γ A hΓ := rfl
+-/
+
+def cases_cons_prop {motive : (Γ : QCtx S) → [NR Γ] → Prop}
+  (h : ∀ (Γ : PCtx S) (A : PTerm S) (h : Nonempty (A :: Γ ⊢ ⬝)), motive ⟦Γ.cons A h⟧)
+  (Γ : QCtx S) [NR Γ] :
+    motive Γ :=
+  Quotient.ind (motive := fun Γ : QCtx S ↦ ([NR Γ] → motive Γ)) (cases_cons' h) Γ
+
+def pb_cons₀ (Δ : QCtx S) (Γ : PCtx S) (A : PTerm S)
+  (h : Nonempty (A :: Γ ⊢ ⬝)) (f : Δ ⟶ ft ⟦Γ.cons A h⟧) :
+    Ctx S where
+  ctx := simulSubst A 0 [f]ᵣ :: [Δ]ᵣ
+  wf := ⟨by
+    apply simulSubst_wf _ ((isMor'_isMor f.is).append A)
+    simp; rw [← List.cons_append]
+    apply append_wf Δ.wf
+      (ctx_betac_wf_cons (choice h) (wf _) (ft_mk_cons_rep_betac _ _ _).symm)⟩
+
+def pb_cons (Δ : QCtx S) (Γ : PCtx S) (A : PTerm S)
+  (h : Nonempty (A :: Γ ⊢ ⬝)) (f : Δ ⟶ ft ⟦Γ.cons A h⟧) :
+    QCtx S :=
+  ⟦pb_cons₀ Δ Γ A h f⟧
+
+lemma heq_aux_func {A B : Sort u} {C : Sort v} (f : A → C) (g : B → C) (h : A = B)
+  (h' : ∀ (a : A) (b : B), HEq a b → f a = g b) :
+    HEq f g := by
+  cases h
+  simp
+  ext c
+  apply h'
+  rfl
+
+def betac_of_heq {A B A' B' : QCtx S} {f : A ⟶ B} {g : A' ⟶ B'}
+  (h₁ : HEq A A') (h₂ : HEq B B') (h₃ : HEq f g) :
+    [f]ᵣ ≃β [g]ᵣ := by
+  cases h₁; cases h₂
+  simp at h₃
+  rw [← Quotient.out_equiv_out] at h₃
+  exact choice h₃
+
+lemma pb_cons_sound (Δ : QCtx S) (Γ Γ' : PCtx S) (A A' : PTerm S)
+  (h : Nonempty (A :: Γ ⊢ ⬝)) (h' : Nonempty (A' :: Γ' ⊢ ⬝)) (eqv : Γ.cons A h ≈ Γ'.cons A' h') :
+    HEq (Δ.pb_cons Γ A h) (Δ.pb_cons Γ' A' h') := by
+  apply heq_aux_func
+  . congr 2; apply Quotient.sound eqv
+  . intro f g hfg
+    rw [← Quotient.out_equiv_out]
+    constructor
+    simp [pb_cons]
+    refine (Ctx.mk_rep_betac _).trans _ _ _ ?_
+    refine PCtx.betac.trans _ _ _ ?_ (Ctx.mk_rep_betac _).symm
+    simp [pb_cons₀]
+    apply betac.of_head_of_eq
+    apply simulSubst_betac (choice eqv).head
+    apply betac_of_heq (HEq.refl _) _ hfg
+    congr 1; apply Quotient.sound eqv
+
+def pb {Γ Δ : QCtx S} [NR Γ] : (f : Δ ⟶ Γ.ft) → QCtx S :=
+  cases_cons (pb_cons Δ) (pb_cons_sound Δ) Γ
+
+@[simp]
+lemma pb_spec {Δ : QCtx S} {Γ : PCtx S} {A : PTerm S}
+  {h : Nonempty (A :: Γ ⊢ ⬝)} {f : Δ ⟶ ft ⟦Γ.cons A h⟧} :
+    pb f = Δ.pb_cons Γ A h f := rfl
+
+/-
+-- error :
+def pb {Γ Δ : QCtx S} [NR Γ] (f : Δ ⟶ Γ.ft) : QCtx S :=
+  cases_cons (pb_cons Δ) (pb_cons_sound Δ) Γ
+-/
+
+def pb_fst_cons₀ (Δ : QCtx S) (Γ : PCtx S) (A : PTerm S) (h : Nonempty (A :: Γ ⊢ ⬝))
+    (f : Δ ⟶ ft ⟦Γ.cons A h⟧) : hom₀ (Δ.pb_cons Γ A h f).out (⟦Γ.cons A h⟧ : QCtx S).out where
+  seq := (#0) :: [f]ᵣ.lift 1 0
+  is := ⟨by
+    have : ((simulSubst A 0 [f]ᵣ) ↑ 1) = simulSubst A 0 ([f]ᵣ ↑↑ 1):= by
+      apply simulSubst_lift
+      simp [← f.is.length_eq, (ft_mk_cons_rep_betac _ _ _).length_eq]
+      apply lift_inv_of_typing (exists_of_cons' (choice h)).snd
+    apply isMor_betac (Ctx.wf' _) (wf _) (Ctx.wf' _) (Ctx.mk_rep_betac _).symm
+      (Ctx.mk_rep_betac _).symm
+    apply isMor.cons
+    apply isMor.weakening_cons (Δ.pb_cons₀ Γ A h f).wf' (wf_of_cons (choice h))
+    apply isMor_betac₂ (wf _) (ft_mk_cons_rep_betac _ _ _) (wf_of_cons (choice h)) f.is
+    simp [pb_cons₀]
+    rw [← this]; apply (weakening_cons_typing (Δ.pb_cons₀ Γ A h f).wf').snd
+    rw [← this]; apply typing.var _ _ _ (Ctx.wf' _) ⟨_, ⟨rfl, isItem.zero _⟩⟩⟩
+
+def pb_fst_cons (Δ : QCtx S) (Γ : PCtx S) (A : PTerm S) (h : Nonempty (A :: Γ ⊢ ⬝))
+  (f : Δ ⟶ ft ⟦Γ.cons A h⟧) :
+    Δ.pb_cons Γ A h f ⟶ ⟦Γ.cons A h⟧ := ⟦Δ.pb_fst_cons₀ Γ A h f⟧
+
+lemma hom_heq_of_betac {Γ Γ' Δ Δ' : QCtx S} (h₁ : Γ = Γ') (h₂ : Δ = Δ')
+  {f : Γ ⟶ Δ} {g : Γ' ⟶ Δ'} (h₃ : [f]ᵣ ≃β [g]ᵣ) :
+    HEq f g := by
+  cases h₁; cases h₂
+  simp; rw [← Quotient.out_equiv_out]
+  exact ⟨h₃⟩
+
+lemma pb_fst_cons_sound (Δ : QCtx S) (Γ Γ' : PCtx S) (A A' : PTerm S)
+  (h : Nonempty (A :: Γ ⊢ ⬝)) (h' : Nonempty (A' :: Γ' ⊢ ⬝)) (eqv : Γ.cons A h ≈ Γ'.cons A' h'):
+    HEq (Δ.pb_fst_cons Γ A h) (Δ.pb_fst_cons Γ' A' h') := sorry
+
+def pb_fst {Γ Δ : QCtx S} [NR Γ] : (f : Δ ⟶ Γ.ft) → (pb f ⟶ Γ) := by
+  apply cases_cons (motive := fun (x : QCtx S) [NR x] ↦ (f : Δ ⟶ x.ft) → (pb f ⟶ x))
+    Δ.pb_fst_cons Δ.pb_fst_cons_sound
+
+@[simp]
+lemma pb_fst_spec {Δ : QCtx S} {Γ : PCtx S} {A : PTerm S}
+  {h : Nonempty (A :: Γ ⊢ ⬝)} {f : Δ ⟶ ft ⟦Γ.cons A h⟧} :
+    pb_fst f = Δ.pb_fst_cons Γ A h f := rfl
+
+lemma gr_pb_cons (Δ : QCtx S) (Γ : PCtx S) (A : PTerm S) (h : Nonempty (A :: Γ ⊢ ⬝))
+  (f : Δ ⟶ ft ⟦Γ.cons A h⟧) :
+    gr (Δ.pb_cons Γ A h f) ≠ 0 := by
+  simp only [gr, pb_cons]
+  rw [(Ctx.mk_rep_betac _).length_eq]
+  simp [pb_cons₀]
+
+lemma gr_pb {Γ Δ : QCtx S} [NR Γ] {f : Δ ⟶ Γ.ft} :
+  gr (pb f) ≠ 0 :=
+  cases_cons_prop (motive := fun (x : QCtx S) [NR x] ↦ {f : Δ ⟶ ft x} → gr (pb f) ≠ 0)
+    (gr_pb_cons Δ) Γ
+
+lemma ft_pb_cons (Δ : QCtx S) (Γ : PCtx S) (A : PTerm S) (h : Nonempty (A :: Γ ⊢ ⬝))
+  (f : Δ ⟶ ft ⟦Γ.cons A h⟧) :
+    (Δ.pb_cons Γ A h f).ft = Δ := by
+  rw [← Quotient.out_equiv_out]
+  exact ⟨(ft_rep_betac_rep_tail _).trans _ _ _ (Ctx.mk_rep_betac _).tail'⟩
+
+lemma ft_pb {Γ Δ : QCtx S} [NR Γ] {f : Δ ⟶ Γ.ft} :
+  ft (pb f) = Δ :=
+  cases_cons_prop (motive := fun (x : QCtx S) [NR x] ↦ {f : Δ ⟶ ft x} → ft (pb f) = Δ)
+    (ft_pb_cons Δ) Γ
+
+lemma isPullback_cons (Δ : QCtx S) (Γ : PCtx S) (A : PTerm S) (h : Nonempty (A :: Γ ⊢ ⬝))
+  (f : Δ ⟶ ft ⟦Γ.cons A h⟧) :
+    IsPullback (Δ.pb_fst_cons Γ A h f)
+      (proj (Δ.pb_cons Γ A h f) ≫ eqToHom (Δ.ft_pb_cons Γ A h f))
+      (proj ⟦Γ.cons A h⟧) f := sorry
+
+lemma isPullback {Γ Δ : QCtx S} [NR Γ] {f : Δ ⟶ Γ.ft} :
+    IsPullback (pb_fst f) (proj (pb f) ≫ eqToHom ft_pb) (proj Γ) f :=
+  cases_cons_prop (motive := fun (x : QCtx S) [NR x] ↦ {f : Δ ⟶ ft x} →
+      IsPullback (pb_fst f) (proj (pb f) ≫ eqToHom ft_pb) (proj x) f) Δ.isPullback_cons Γ
+
+lemma pullback_id_obj_cons (Γ : PCtx S) (A : PTerm S) (h : Nonempty (A :: Γ ⊢ ⬝)) :
+    pb_cons _ Γ A h (𝟙 _) = ⟦Γ.cons A h⟧ := by
+  apply Quotient.sound
+  constructor
+  apply betac.of_head_of_tail _ (ft_mk_cons_rep_betac Γ A h)
+  refine (id_rep_betac _).simulSubst.trans _ _ _ ?_
+  simp [id, id₀]
+  erw [(ft_mk_cons_rep_betac Γ _ _).length_eq, simulSubst_id_cons (choice h)]
+  apply betac.refl _
+
+lemma pullback_id_obj {Γ : QCtx S} [NR Γ] :
+    pb (𝟙 (ft Γ)) = Γ :=
+  cases_cons_prop (motive := fun (x : QCtx S) [NR x] ↦ pb (𝟙 (ft x)) = x) pullback_id_obj_cons Γ
+
+lemma _root_.CategoryTheory.eqToHom_comp_eq_iff {C : Type u₁} [CategoryTheory.Category.{u₂, u₁} C]
+  {X X' Y : C} (f : X' ⟶ Y) (g : X ⟶ Y) (h : X = X') :
+    eqToHom h ≫ f = g ↔ HEq f g := by
+  constructor
+  all_goals cases h; simp
+
+lemma pullback_id_map_cons (Γ : PCtx S) (A : PTerm S) (h : Nonempty (A :: Γ ⊢ ⬝)) :
+    eqToHom (pullback_id_obj_cons Γ A h).symm ≫ pb_fst (𝟙 (ft ⟦Γ.cons A h⟧)) = 𝟙 _ := by
+  rw [eqToHom_comp_eq_iff]
+  apply hom_heq_of_betac (pullback_id_obj_cons Γ A h) rfl
+  simp [pb_fst_cons]
+  refine ((hom₀.mk_rep_betac _).trans _ _ _ ?_).trans _ _ _ (id_rep_betac _).symm
+  simp [pb_fst_cons₀]
+  refine (PCtx.betac.of_tail_of_eq (id_rep_betac _).lift).trans _ _ _ ?_
+  simp [id, id₀]
+  rw [(ft_mk_cons_rep_betac Γ _ _).length_eq, (Ctx.mk_rep_betac _).length_eq]
+  simp only [idN, zero_add]
+  rw [idN_lift (by simp)]
+  apply PCtx.betac.refl _
+
+lemma pullback_id_map {Γ : QCtx S} [NR Γ] :
+    eqToHom pullback_id_obj.symm ≫ pb_fst (𝟙 (ft Γ)) = 𝟙 Γ :=
+  cases_cons_prop (motive := fun (x : QCtx S) [NR x] ↦
+    (eqToHom pullback_id_obj.symm ≫ pb_fst (𝟙 (ft x)) = 𝟙 x)) pullback_id_map_cons Γ
+
+#check ContextualCategory.pullback_comp_obj
+
+instance NR_pb {Δ Γ : QCtx S} [NR Γ] {f : Δ ⟶ ft Γ} :
+    NR (pb f) := ⟨gr_pb⟩
+
+lemma pullback_comp_obj_cons (Δ Θ : QCtx S) (Γ : PCtx S) (A : PTerm S)
+  (h : Nonempty (A :: Γ ⊢ ⬝)) (f : Δ ⟶ ft ⟦Γ.cons A h⟧) (g : θ ⟶ Δ) :
+    pb (g ≫ f) = pb (g ≫ eqToHom (ft_pb (f := f).symm)) := by
+  apply Quotient.sound
+  constructor
+  apply betac.of_head_of_eq
+  rw [← simulSubst_pcomp (exists_of_cons' (choice h)).snd (hom.is _) _ (isTrunc.zero _)]
+  apply PCtx.betac.simulSubst
+  refine (hom₀.mk_rep_betac _).trans _ _ _ ?_
+  simp [comp₀]
+  apply pcomp_betac₁ $ betac_of_heq (by rfl) (by simp [ft_pb_cons])
+    (by simp only [heq_comp_eqToHom_iff, heq_eq_eq])
+  rw [ft_pb]
+  apply isMor_betac₂ (Ctx.wf' _) (ft_mk_cons_rep_betac Γ A h) (wf_of_cons (choice h)) f.is
+
+lemma pullback_comp_obj {Γ Δ Θ : QCtx S} [NR Γ] {f : Δ ⟶ ft Γ} {g : Θ ⟶ Δ}:
+    pb (g ≫ f) = pb (g ≫ eqToHom (ft_pb (f := f)).symm) :=
+  cases_cons_prop (motive := fun (x : QCtx S) [NR x] ↦ {f : Δ ⟶ ft x} → {g : Θ ⟶ Δ} →
+    pb (g ≫ f) = pb (g ≫ eqToHom (ft_pb (f := f)).symm)) (pullback_comp_obj_cons Δ Θ) Γ
+
+
+
+/-
+instance : ContextualCategory (QCtx S) where
+  pb := _
+  pb_fst := _
+  gr_pb := _
+  ft_pb := _
+  isPullback := _
+  pullback_id_obj := _
+  pullback_id_map := _
+  pullback_comp_obj := _
+  pullback_comp_map := _
+-/
+
+end QCtx
+
+end TermModel
